src/Node.v
@@ -1,0 +1,120 @@
+Require Import Coq.Structures.OrderedType.
+Require Import Coq.Structures.OrderedTypeEx.
+Require Import Coq.FSets.FMapAVL.
+Require Import Coq.FSets.FSetAVL.
+Require Import Coq.Arith.Peano_dec.
+Require Import Aniceto.Map.
+
+Require Coq.FSets.FMapFacts.
+
+Require Import Tid.
+
+Structure node := {
+  n_task: tid;
+  n_id: nat
+}.
+
+Definition zero t := {| n_task := t; n_id:= 0 |}.
+
+
+Module NODE <: OrderedType.
+  Definition t := node.
+  Definition eq := @eq node.
+  Definition lt n1 n2 := n_id n1 < n_id n2 \/ (n_id n1 = n_id n2 /\ TID.lt (n_task n1) (n_task n2)).
+
+  Lemma eq_refl:
+    forall x,
+    eq x x.
+  Proof.
+    unfold eq; trivial.
+  Qed.
+
+  Lemma eq_sym:
+    forall x y,
+    eq x y ->
+    eq y x.
+  Proof.
+    unfold eq; auto.
+  Qed.
+
+  Lemma eq_trans :
+    forall x y z,
+    eq x y ->
+    eq y z ->
+    eq x z.
+  Proof.
+    unfold eq.
+    intros; subst; trivial.
+  Qed.
+
+  Lemma lt_trans:
+    forall x y z : t, lt x y -> lt y z -> lt x z.
+  Proof.
+    unfold lt.
+    intros.
+    destruct H as [?|(?,?)], H0 as [?|(?,?)]; eauto using TID.lt_trans with *.
+  Qed.
+
+  Lemma lt_not_eq : forall x y : t, lt x y -> ~ eq x y.
+  Proof.
+    unfold eq, lt.
+    intros.
+    destruct H as [?|(?,?)].
+    - intuition; subst; auto with *.
+    - intuition; subst.
+      apply TID.lt_not_eq in H0.
+      eauto using TID.lt_not_eq with *.
+  Qed.
+
+  Require Import Coq.Structures.OrderedTypeEx.
+  Require Import Coq.Arith.Compare_dec.
+  Lemma compare:
+    forall x y, Compare lt eq x y.
+  Proof.
+    intros.
+    unfold lt.
+    destruct (Nat_as_OT.compare (n_id x) (n_id y));
+    unfold Nat_as_OT.lt, Nat_as_OT.eq in *;
+    auto using LT, GT.
+    destruct (TID.compare (n_task x) (n_task y));
+    auto using LT, GT. 
+    destruct x, y.
+    unfold TID.eq in *.
+    simpl in *; subst.
+    apply EQ.
+    unfold eq; auto.
+  Qed.
+
+  Lemma eq_dec : forall x y : t, {eq x y} + {~ eq x y}.
+  Proof.
+    intros.
+    unfold eq.
+    destruct x as (x1,x2), y as (y1,y2).
+    destruct (tid_eq_dec x1 y1), (eq_nat_dec x2 y2); subst; eauto;
+      right;
+      intuition;
+      inversion H; subst;
+      contradiction n; auto.
+  Qed.
+
+End NODE.
+
+Lemma node_eq_rw:
+  forall x y, NODE.eq x y <-> x = y.
+Proof.
+  unfold NODE.eq; intuition. 
+Qed.
+
+Lemma node_eq_dec:
+  forall (x y:node),
+  { x = y } + { x <> y }.
+Proof.
+  intros.
+  destruct (NODE.eq_dec x y); rewrite node_eq_rw in *; auto.
+Qed.
+
+Module MN := FMapAVL.Make NODE.
+Module MN_Facts := FMapFacts.Facts MN.
+Module MN_Props := FMapFacts.Properties MN.
+Module MN_Extra := MapUtil MN.
+
